verif/btrees_spec.v
@@ -133,15 +133,13 @@ Definition moveToFirst_spec : ident * funspec :=
   DECLARE _moveToFirst
   WITH r:relation val, pr:val, c:cursor val, pc:val, n:node val, pn:val
   PRE[ _node OF tptr tbtnode, _cursor OF tptr tcursor, _level OF tint ]
-  PROP(cursor_correct c n (get_root r); cursor_wf c; pn = getval n)
+  PROP(partial_cursor_correct c n (get_root r); cursor_wf c; pn = getval n)
   LOCAL(temp _cursor pc; temp _node pn; temp _level (Vint(Int.repr(Zlength c))))
   SEP(relation_rep r pr; cursor_rep c r pc)
   POST[ tvoid ]
   PROP()
   LOCAL()
-  SEP(relation_rep r pr; cursor_rep (moveToFirst n c (length c)) r pc).
-  
-                                                                    
+  SEP(relation_rep r pr; cursor_rep (moveToFirst n c (length c)) r pc).                                 
                                                                       
 (**
     GPROG
